Proved some cases of a key lemma about allocating a new algebraic datatype node

platform/Depl/AlgebraicDatatypes.v
@@ -11,6 +11,8 @@ Require Import Depl.Logic.
 
 (** One constructor of a datatype *)
 Record con := {
+  Name : string;
+  (* Identifier for this constructor, to use in executable code *)
   Recursive : list string;
   (** Names for the "record fields" that actually exist at runtime,
     * referencing other objects of this same datatype.
@@ -22,10 +24,11 @@ Record con := {
   Condition : pred
   (** Finally, the property describing associated memory resources.
     * It does _not_ describe the transitive conditions imposed by other values of the same algebraic
-    * datatype that this node points to. *)
+    * datatype that this node points to.
+    * A variable "this" is available to refer to the model of this node. *)
 }.
 
-Definition datatype := list con.
+Definition datatype := (string * list con)%type.
 
 
 (** * Semantics of datatypes *)
@@ -37,6 +40,8 @@ Inductive skeleton :=
 Section Semantics.
   Open Scope Sep_scope.
 
+  Variable hO : ho_env nil.
+
   (** We'll represent recursive arguments as pairs of models and pointers.
     * Here are some functions to disentangle them. *)
   Definition addrs : list (dyn * W) -> list W := map (@snd _ _).
@@ -46,11 +51,11 @@ Section Semantics.
   Definition dynify : list W -> list dyn := map (@Dyn _).
 
   (** Helpers for building first-order variable environments *)
-  Fixpoint make_fo (names : list string) (values : list dyn) : fo_env :=
+  Fixpoint make_fo (names : list string) (values : list dyn) (base : fo_env) : fo_env :=
     match names, values with
       | name :: names, valu :: values =>
-        fo_set (make_fo names values) name valu
-      | _, _ => fo_empty
+        fo_set (make_fo names values base) name valu
+      | _, _ => base
     end.
 
   Section children.
@@ -75,13 +80,13 @@ Section Semantics.
       (* There exist values for the recursive and nonrecursive fields... *)
       Ex rs, Ex ns,
         (* Laid out at the appropriate address, we find the tag and arguments. *)
-        ptsto32m _ ptr O (tag :: addrs rs ++ ns)
+        ptsto32m _ ptr O (tag :: ns ++ addrs rs)
         (* We picked the right number of fields in each category. *)
         * [| length rs = length (Recursive c) |]
         * [| length ns = length (Nonrecursive c) |]
         (* The side condition holds w.r.t. the field values. *)
-        * predD (Condition c) (fun _ _ => Emp)
-        (make_fo (Recursive c ++ Nonrecursive c) (models rs ++ dynify ns))
+        * predD (Condition c) hO
+        (make_fo ("this" :: Recursive c ++ Nonrecursive c) (model :: models rs ++ dynify ns) fo_empty)
         (* Finally, all child nodes are accounted for. *)
         * children sks rs.
   End children.
@@ -94,8 +99,264 @@ Section Semantics.
     match sk with
       | Skeleton sks =>
         (** It turned out to be the [n]th constructor, whose definition is [c]... *)
-        Ex n, Ex c, [| nth_error dt n = Some c |]
+        Ex n, Ex c, [| nth_error (snd dt) n = Some c |]
           (* ...and this node is sitting in memory where we expect it. *)
           * conD datatypeD c n sks model ptr
     end.
 End Semantics.
+
+
+(** * Normalized datatype definitions *)
+
+Record ncon := {
+  NName : string;
+  NRecursive : list string;
+  NNonrecursive : list string;
+  NCondition : normal
+}.
+
+Definition ndatatype := (string * list ncon)%type.
+
+Definition normalizeCon (c : con) : ncon := {|
+  NName := Name c;
+  NRecursive := Recursive c;
+  NNonrecursive := Nonrecursive c;
+  NCondition := normalize (Condition c)
+|}.
+
+Definition normalizeDatatype (dt : datatype) : ndatatype :=
+  (fst dt, map normalizeCon (snd dt)).
+
+
+(** * Functions to construct key formulas related to constructing and deconstructing datatype values *)
+
+(** Multiple substitution for first-order variables, recording where we left off in eating arguments *)
+Fixpoint nsubsts (xs : list fo_var) (args : list expr) (n : normal) : normal * list expr :=
+  match xs, args with
+    | x :: xs', e :: args' => nsubsts xs' args' (nsubst x e n)
+    | _, _ => (n, args)
+  end.
+
+(** Constructing recursive subgoals for the recursive arguments of a constructor *)
+Fixpoint recursives (dtName : string) (xs : list fo_var) (args : list expr) : list pred :=
+  match xs, args with
+    | x :: xs', e :: args' => Named dtName (Var x :: e :: nil) :: recursives dtName xs' args'
+    | _, _ => nil
+  end.
+
+(** What chunk of state do we expect to see associated with arguments to a new construction? *)
+Definition allocatePre (dtName : string) (c : ncon) (args : list expr) : normal :=
+  let (cond, recs) := nsubsts (NNonrecursive c) args (NCondition c) in
+  {|
+    NQuants := NRecursive c ++ NQuants cond;
+    NPure := NPure cond;
+    NImpure := recursives dtName (NRecursive c) recs ++ NImpure cond
+  |}.
+
+Section allocatePre_sound.
+  Variable dt : datatype.
+  Variable tag : nat.
+  Variable c : con.
+
+  Hypothesis Htag : nth_error (snd dt) tag = Some c.
+  (* The constructor we think we're using really is found at the right position in the type defn. *)
+
+  Variable hE : ho_env nil.
+
+  Hypothesis HhE_fwd : forall m p, hE (fst dt) (m :: Dyn p :: nil)
+    ===> (Ex sk, datatypeD hE dt sk m p).
+  Hypothesis HhE_bwd : forall m p, (Ex sk, datatypeD hE dt sk m p)
+    ===> hE (fst dt) (m :: Dyn p :: nil).
+  (* The higher-order variable environment is interpreting this datatype's name in the proper way. *)
+
+  Lemma allocatePre_sound' : forall fvs bvs,
+    wellScoped fvs (Condition c)
+    -> boundVars (Condition c) = Some bvs
+    -> (forall x, In x bvs -> ~In x fvs)
+    -> NoDup (Recursive c)
+    -> (forall x, In x (Recursive c) -> ~In x bvs)
+    -> (forall x, In x (Recursive c) -> ~In x fvs)
+    -> forall args fE ws, length args = length (Nonrecursive c) + length (Recursive c)
+    -> map (fun e => exprD e fE) args = map (@Dyn W) ws
+    -> (forall fE1 fE2, (forall x, ~In x (Recursive c) -> ~In x bvs -> fE1 x = fE2 x)
+      -> List.Forall (fun e => exprD e fE1 = exprD e fE2) args)
+    -> normalD (allocatePre (fst dt) (normalizeCon c) args) hE fE
+    ===> Ex sks, Ex rs, [| length rs = length (Recursive c) |]
+    * children (datatypeD hE dt) sks rs
+    * predD (Condition c) hE
+    (make_fo (Recursive c ++ Nonrecursive c)
+      (models rs ++ dynify (firstn (length (Recursive c)) ws)) fE).
+  Proof.
+    destruct c; simpl in *.
+    clear Htag.
+    intros until args; generalize dependent Recursive0; generalize dependent Nonrecursive0;
+      generalize dependent Condition0;
+      induction args; unfold allocatePre; simpl; intros.
+
+    destruct Nonrecursive0; simpl in *; try discriminate.
+    destruct Recursive0; simpl in *; try discriminate.
+    apply Himp_ex_c; exists nil.
+    apply Himp_ex_c; exists nil.
+    simpl.
+    eapply Himp_trans; [ | apply Himp_star_assoc' ].
+    apply Himp_star_pure_cc; auto.
+    eapply Himp_trans; [ | apply Himp_star_Emp' ].
+    apply addSubstsH.
+    eapply normalize_sound_bwd; eauto.
+    unfold not in *; eauto.
+
+    destruct Nonrecursive0; simpl in *; intros.
+
+    destruct Recursive0; simpl in *; try discriminate.
+    injection H5; clear H5; intros.
+    unfold allocatePre in IHargs; simpl in IHargs.
+    specialize (IHargs Condition0 H H0 nil Recursive0); simpl in IHargs; intuition.
+    apply Himp'_ex; fold addQuants; simpl; intro r.
+    eapply Himp_trans; [ apply addSubstsH; apply addQuants_monotone | ].
+    intros.
+    apply star_out_fwd.
+    destruct ws; simpl in *; try discriminate.
+    injection H6; clear H6; intros.
+    inversion_clear H2.
+
+    Lemma addQuants_push_fwdPlus : forall f p qs fE,
+      (forall fE1 fE2, (forall x, ~In x qs -> fE1 x = fE2 x) -> p fE1 = p fE2)
+      -> addQuants qs (fun fE' : fo_env => p fE' * f fE') fE ===>
+      p fE * addQuants qs f fE.
+    Proof.
+      induction qs; simpl; intuition.
+
+      apply Himp_refl.
+
+      apply Himp'_ex; intro y.
+      eapply Himp_trans; [ apply IHqs; eauto | ].
+      apply Himp_star_frame.
+      apply Himp_refl'.
+      apply H; intros.
+      unfold fo_set.
+      destruct (string_dec x a); intuition.
+      apply Himp_ex_c; exists y; apply Himp_refl.
+    Qed.
+
+    eapply Himp_trans; [ apply addQuants_push_fwdPlus | ].
+    intros.
+    do 2 f_equal.
+    apply H2; intro.
+    apply in_app_or in H11; intuition eauto using normalize_boundVars.
+    f_equal.
+    specialize (H7 fE1 fE2).
+    match type of H7 with
+      | ?P -> _ => assert P
+    end.
+    intuition idtac.
+    apply H2; intro.
+    apply in_app_or in H12; intuition eauto using normalize_boundVars.
+    intuition idtac.
+    inversion H13; auto.
+
+    simpl.
+    assert (Hscoped : forall fE1 fE2,
+      (forall x, (s = x \/ In x Recursive0 -> False) ->
+        (In x bvs -> False) -> fE1 x = fE2 x)
+       -> List.Forall (fun e => exprD e fE1 = exprD e fE2) args).
+    intros.
+    specialize (H7 fE1 fE2); intuition idtac.
+    inversion H12; auto.
+
+    Theorem map_same : forall A B (f g : A -> B) ls,
+      List.Forall (fun x => f x = g x) ls
+      -> map f ls = map g ls.
+    Proof.
+      induction 1; simpl; intuition.
+    Qed.
+
+    eapply Himp_trans; [ apply Himp_star_frame; [ apply Himp_refl | apply IHargs; eauto ] | ].
+    erewrite map_same.
+    eassumption.
+    simpl.
+    eapply Forall_weaken; [ | apply Hscoped ].
+    simpl; eauto; intros.
+    intros; unfold fo_set.
+    destruct (string_dec x s); intuition subst; tauto.
+
+    replace (exprD a (fo_set fE s r)) with (exprD a fE).
+    rewrite H8.
+    eapply Himp_trans; [ apply Himp_star_frame; [ apply HhE_fwd | apply Himp_refl ] | ].
+    eapply Himp_trans; [ apply Himp_ex_star | ].
+    apply Himp'_ex; intro sk.
+    eapply Himp_trans; [ apply Himp_star_comm | ].
+    eapply Himp_trans; [ apply Himp_ex_star | ].
+    apply Himp'_ex; intro sks.
+    eapply Himp_trans; [ apply Himp_ex_star | ].
+    apply Himp'_ex; intro rs.
+    apply Himp_ex_c; exists (sk :: sks).
+    apply Himp_ex_c; exists ((r, w) :: rs).
+    simpl.
+    rewrite <- app_nil_end.
+    unfold fo_set at 2.
+    destruct (string_dec s s); try tauto.
+
+    Lemma make_fo_unused : forall base values' values names,
+      length values = length names
+      -> make_fo names (values ++ values') base = make_fo names values base.
+    Proof.
+      induction values; destruct names; simpl; intuition.
+      f_equal; auto.
+    Qed.
+
+    eapply Himp_trans; [ apply Himp_star_frame; [ apply Himp_star_assoc | apply Himp_refl ] | ].
+    eapply Himp_trans; [ apply Himp_star_assoc |  ].
+    apply Himp_star_pure_c; intro.
+    repeat rewrite make_fo_unused by (unfold models; rewrite map_length; auto).
+    eapply Himp_trans; [ | apply Himp_star_assoc' ].
+    apply Himp_star_pure_cc; auto.
+    assert (predD Condition0 hE (make_fo Recursive0 (models rs) (fo_set fE s r))
+      ===> predD Condition0 hE (fo_set (make_fo Recursive0 (models rs) fE) s r)).
+    apply addSubstsH.
+    eapply weaken_predD; eauto; intros.
+    
+    Lemma make_fo_reorder : forall s r x xs vs fE,
+      ~In s xs
+      -> make_fo xs vs (fo_set fE s r) x = fo_set (make_fo xs vs fE) s r x.
+    Proof.
+      induction xs; destruct vs; simpl; intuition.
+      unfold fo_set at 1 3.
+      destruct (string_dec x a); subst.
+      destruct (string_dec a s); subst.
+      tauto.
+      unfold fo_set.
+      destruct (string_dec a a); tauto.
+      destruct (string_dec x s); subst.
+      rewrite IHxs by auto.
+      unfold fo_set.
+      destruct (string_dec s s); tauto.
+      rewrite IHxs by auto.
+      unfold fo_set.
+      destruct (string_dec x s); intuition.
+      destruct (string_dec x a); intuition.
+    Qed.
+
+    apply make_fo_reorder; auto.
+      
+    generalize H11; clear.
+    generalize (datatypeD hE dt); intro.
+    generalize (children h); intro.
+    generalize (predD Condition0 hE); intro.
+    sepLemma.
+
+    specialize (H7 fE (fo_set fE s r)).
+    match type of H7 with
+      | ?P -> _ => assert P
+    end.
+    intuition idtac.
+    unfold fo_set.
+    destruct (string_dec x s); subst; auto; tauto.
+    intuition idtac.
+    inversion H12; auto.
+
+
+    (** Case where recursive args are exhausted and we start on the nonrecursives *)
+    admit.
+  Qed.
+
+End allocatePre_sound.
